module Duration where

open import Data.Rational as Rat using (â„š; 0â„š; 1â„š)
import Data.Rational.Properties as Rat
open import Data.Integer using (+â‰¤+; +_; +[1+_]; -[1+_])
open import Data.Nat using (â„•; zero; suc; zâ‰¤n; sâ‰¤s)
open import Relation.Binary.PropositionalEquality


record ğ”» : Set where
  constructor mkDur
  field
    duration : â„š
    positive : 0â„š Rat.â‰¤ duration

infix 4 _â‰¤_ _<_

_â‰¤_ : ğ”» â†’ ğ”» â†’ Set
x â‰¤ y = ğ”».duration x Rat.â‰¤ ğ”».duration y

_<_ : ğ”» â†’ ğ”» â†’ Set
x < y = ğ”».duration x Rat.< ğ”».duration y

open import Data.Unit using (tt)

infixr 5 _+_
_+_ : ğ”» â†’ ğ”» â†’ ğ”»
mkDur dâ‚ pâ‚ + mkDur dâ‚‚ pâ‚‚ = mkDur (dâ‚ Rat.+ dâ‚‚) (Rat.+-mono-â‰¤ pâ‚ pâ‚‚)

infixr 6 _âŠ”_ _âŠ“_ _*_

_âŠ”_ : ğ”» â†’ ğ”» â†’ ğ”»
mkDur dâ‚ pâ‚ âŠ” mkDur dâ‚‚ pâ‚‚ = mkDur (dâ‚ Rat.âŠ” dâ‚‚) (Rat.âŠ”-mono-â‰¤ pâ‚ pâ‚‚)

_âŠ“_ : ğ”» â†’ ğ”» â†’ ğ”»
mkDur dâ‚ pâ‚ âŠ“ mkDur dâ‚‚ pâ‚‚ = mkDur (dâ‚ Rat.âŠ“ dâ‚‚) (Rat.âŠ“-mono-â‰¤ pâ‚ pâ‚‚)

_*_ : ğ”» â†’ ğ”» â†’ ğ”»
mkDur dâ‚ pâ‚ * mkDur dâ‚‚ pâ‚‚ = mkDur (dâ‚ Rat.* dâ‚‚) ( begin
  0â„š Rat.* 0â„š  â‰¤âŸ¨ Rat.*-monoÊ³-â‰¤-nonNeg 0â„š tt pâ‚ âŸ©
  dâ‚ Rat.* 0â„š  â‰¤âŸ¨ Rat.*-monoË¡-â‰¤-nonNeg dâ‚ (Rat.nonNegative pâ‚) pâ‚‚ âŸ©
  dâ‚ Rat.* dâ‚‚  âˆ)
  where open Rat.â‰¤-Reasoning

0ğ”» : ğ”»
0ğ”» = mkDur 0â„š Rat.â‰¤-refl

1ğ”» : ğ”»
1ğ”» = mkDur 1â„š (Rat._â‰¤_.*â‰¤* (+â‰¤+ zâ‰¤n))

fromâ„• : â„• â†’ ğ”»
fromâ„• zero = 0ğ”»
fromâ„• (â„•.suc x) = 1ğ”» + fromâ„• x

_â»Â¹ : ğ”» â†’ ğ”»
mkDur (Rat.mkâ„š (+ zero) d isCoprime) p â»Â¹ = 0ğ”»
mkDur r@(Rat.mkâ„š +[1+ n ] d isCoprime) p â»Â¹ = mkDur (Rat.1/ r) (Rat._â‰¤_.*â‰¤* (+â‰¤+ zâ‰¤n))
mkDur (Rat.mkâ„š (-[1+_] n) d isCoprime) (Rat._â‰¤_.*â‰¤* ()) â»Â¹

postulate
  â»Â¹âˆ˜â»Â¹ : âˆ€ m â†’ (m â»Â¹) â»Â¹ â‰¡ m
-- â»Â¹âˆ˜â»Â¹ (mkDur r@(Rat.mkâ„š (+_ zero) d isCoprime) positive) = {! !}
-- â»Â¹âˆ˜â»Â¹ (mkDur r@(Rat.mkâ„š +[1+ n ] d isCoprime) positive) = {! !}
-- â»Â¹âˆ˜â»Â¹ (mkDur (Rat.mkâ„š (-[1+_] n) d isCoprime) (Rat.*â‰¤* ()))

_/_ : ğ”» â†’ ğ”» â†’ ğ”»
x / y = x * y â»Â¹

postulate
  *-identityÊ³ : âˆ€ x â†’ x * 1ğ”» â‰¡ x


â‰¤-refl : {x : ğ”»} â†’ x â‰¤ x
â‰¤-refl = Rat.â‰¤-refl

â‰¤-trans : {x y z : ğ”»} â†’ x â‰¤ y â†’ y â‰¤ z â†’ x â‰¤ z
â‰¤-trans = Rat.â‰¤-trans

0ğ”»â‰¤n : {x : ğ”»} â†’ 0ğ”» â‰¤ x
0ğ”»â‰¤n {mkDur duration positive} = positive

sub : (x y : ğ”») â†’ y â‰¤ x â†’ ğ”»
sub (mkDur x px) (mkDur y py) yâ‰¤x = mkDur (x Rat.- y)
  ( begin
  0â„š                 â‰¡âŸ¨ sym (Rat.+-inverseÊ³ x) âŸ©
  x Rat.+ (Rat.- x)  â‰¤âŸ¨ Rat.+-monoÊ³-â‰¤ x (Rat.neg-antimono-â‰¤ yâ‰¤x) âŸ©
  x Rat.+ (Rat.- y)  âˆ
  )
  where open Rat.â‰¤-Reasoning

+-monoË¡-â‰¤ : (r : ğ”») â†’ {lâ‚€ lâ‚ : ğ”»} â†’ lâ‚€ â‰¤ lâ‚ â†’ lâ‚€ + r â‰¤ lâ‚ + r
+-monoË¡-â‰¤ r lâ‰¤l = Rat.+-monoË¡-â‰¤ (ğ”».duration r) lâ‰¤l

+-monoÊ³-â‰¤ : (r : ğ”») â†’ {lâ‚€ lâ‚ : ğ”»} â†’ lâ‚€ â‰¤ lâ‚ â†’ r + lâ‚€ â‰¤ r + lâ‚
+-monoÊ³-â‰¤ r lâ‰¤l = Rat.+-monoÊ³-â‰¤ (ğ”».duration r) lâ‰¤l

sub-mono-â‰¤ : (x y m : ğ”») â†’ (mâ‰¤x : m â‰¤ x) â†’ (mâ‰¤y : m â‰¤ y) â†’ (x â‰¤ y) â†’ sub x m mâ‰¤x â‰¤ sub y m mâ‰¤y
sub-mono-â‰¤ x y m mâ‰¤x mâ‰¤y xâ‰¤y = Rat.+-monoË¡-â‰¤ (Rat.- ğ”».duration m) xâ‰¤y

xâŠ“yâ‰¤xâŠ”y : (x y : ğ”») â†’ x âŠ“ y â‰¤ x âŠ” y
xâŠ“yâ‰¤xâŠ”y x y = Rat.pâŠ“qâ‰¤pâŠ”q (ğ”».duration x) (ğ”».duration y)

open import Relation.Nullary

_â‰Ÿ_ : (x y : ğ”») â†’ Dec (x â‰¡ y)
x â‰Ÿ y with ğ”».duration x Rat.â‰Ÿ ğ”».duration y
(mkDur .duration p â‰Ÿ mkDur duration pâ‚) | yes refl rewrite Rat.â‰¤-irrelevant p pâ‚ = yes refl
... | no z = no Î» { xâ‚ â†’ z (cong ğ”».duration xâ‚) }

_â‰¤?_ : (x y : ğ”») â†’ Dec (x â‰¤ y)
x â‰¤? y = ğ”».duration x Rat.â‰¤? ğ”».duration y

<â‡’â‰¤ : (x y : ğ”») â†’ x < y â†’ x â‰¤ y
<â‡’â‰¤ _ _ = Rat.<â‡’â‰¤

open import Relation.Binary.Definitions using (Trichotomous; tri<; triâ‰ˆ; tri>) public

postulate
  <-cmp : Trichotomous _â‰¡_ _<_
-- <-cmp x y with Rat.<-cmp (ğ”».duration x) (ğ”».duration y)
-- ... | tri< a Â¬b Â¬c = tri< {! !} ? ?
-- ... | triâ‰ˆ Â¬a b Â¬c = triâ‰ˆ {! !} ? ?
-- ... | tri> Â¬a Â¬b c = tri> {! !} ? ?


module â‰¤-Reasoning where
  open Rat.â‰¤-Reasoning public


2ğ”» = 1ğ”» + 1ğ”»
3ğ”» = 2ğ”» + 1ğ”»
4ğ”» = 3ğ”» + 1ğ”»

